pkvm_refinedc/_build/default/src/proofs/check_pkvm_pgtables/generated_spec.v
@@ -1,5 +1,6 @@
 From refinedc.typing Require Import typing.
 From refinedc.project.pkvm_refinedc.src.check_pkvm_pgtables Require Import generated_code.
+From refinedc.project.pkvm_refinedc.src.check_pkvm_pgtables Require Import page_table_entry_type.
 Set Default Proof Using "Type".
 
 (* Generated from [src/check_pkvm_pgtables.c]. *)
@@ -8,7 +9,10 @@ Section spec.
 
   (* Type definitions. *)
 
-  (* Function [entry_kind] has been skipped. *)
+  (* Specifications for function [entry_kind]. *)
+  Definition type_of_entry_kind :=
+    fn(∀ (npte, nlevel) : nat * nat; (npte @ (int (u64))), (nlevel @ (int (u8))); True)
+      → ∃ () : (), (int (u32)); True.
 
   (* Function [hyp_phys_to_virt] has been skipped. *)
 
