pkvm_refinedc/_build/default/src/proofs/check_pkvm_pgtables/generated_proof_entry_kind.v
@@ -1,1 +1,27 @@
-(* You were too lazy to even write a spec for this function. *)
+From refinedc.typing Require Import typing.
+From refinedc.project.pkvm_refinedc.src.check_pkvm_pgtables Require Import generated_code.
+From refinedc.project.pkvm_refinedc.src.check_pkvm_pgtables Require Import generated_spec.
+From refinedc.project.pkvm_refinedc.src.check_pkvm_pgtables Require Import page_table_entry_type.
+Set Default Proof Using "Type".
+
+(* Generated from [src/check_pkvm_pgtables.c]. *)
+Section proof_entry_kind.
+  Context `{!typeG Σ} `{!globalG Σ}.
+
+  (* Typing proof for [entry_kind]. *)
+  Lemma type_entry_kind :
+    ⊢ typed_function impl_entry_kind type_of_entry_kind.
+  Proof.
+    Open Scope printing_sugar.
+    start_function "entry_kind" ([npte nlevel]) => arg_pte arg_level.
+    split_blocks ((
+      ∅
+    )%I : gmap label (iProp Σ)) ((
+      ∅
+    )%I : gmap label (iProp Σ)).
+    - repeat liRStep; liShow.
+      all: print_typesystem_goal "entry_kind" "#0".
+    Unshelve. all: sidecond_hook; prepare_sideconditions; normalize_and_simpl_goal; try solve_goal; unsolved_sidecond_hook.
+    all: print_sidecondition_goal "entry_kind".
+  Qed.
+End proof_entry_kind.
